devel/Iron/SystemF2Effect/Type/Predicate/Wf.v
@@ -4,67 +4,58 @@ Require Export Iron.SystemF2Effect.Kind.
 
 
 (* Well formed types are closed under the given kind environment. *)
-Inductive wfT (kn: nat) : ty -> Prop :=
+Inductive WfT (kn: nat) : ty -> Prop :=
  | WfT_TVar 
    :  forall ki
    ,  ki < kn
-   -> wfT kn (TVar ki)
+   -> WfT kn (TVar ki)
 
  | WfT_TForall
    :  forall k t
-   ,  wfT (S kn) t
-   -> wfT kn (TForall k t)
+   ,  WfT (S kn) t
+   -> WfT kn (TForall k t)
 
  | WfT_TApp
    :  forall t1 t2
-   ,  wfT kn t1 -> wfT kn t2
-   -> wfT kn (TApp t1 t2)
+   ,  WfT kn t1 -> WfT kn t2
+   -> WfT kn (TApp t1 t2)
 
  | WfT_TSum
    :  forall t1 t2
-   ,  wfT kn t1 -> wfT kn t2
-  ->  wfT kn (TSum t1 t2)
+   ,  WfT kn t1 -> WfT kn t2
+  ->  WfT kn (TSum t1 t2)
 
  | WfT_TBot
    :  forall k
-   ,  wfT kn (TBot k)
+   ,  WfT kn (TBot k)
 
  | WfT_TCon0
    :  forall tc
-   ,  wfT kn (TCon0 tc)
+   ,  WfT kn (TCon0 tc)
 
  | WfT_TCon1 
    :  forall tc t1
-   ,  wfT kn t1
-   -> wfT kn (TCon1 tc t1)
+   ,  WfT kn t1
+   -> WfT kn (TCon1 tc t1)
 
  | WfT_TCon2 
    :  forall tc t1 t2
-   ,  wfT kn t1 -> wfT kn t2
-   -> wfT kn (TCon2 tc t1 t2)
+   ,  WfT kn t1 -> WfT kn t2
+   -> WfT kn (TCon2 tc t1 t2)
 
  | WfT_TCap
    :  forall tc
-   ,  wfT kn (TCap tc).
+   ,  WfT kn (TCap tc).
+Hint Constructors WfT.
 
-Hint Constructors wfT.
-
-
-(******************************************************************************)
-(* Closed types are well formed under an empty environment. *)
-Definition closedT : ty -> Prop
- := wfT O.
-Hint Unfold closedT.
+Notation ClosedT := (WfT 0).
 
 
 Lemma closedT_tRef
  :  forall r1 t2
- ,  closedT t2
- -> closedT (tRef (TCap (TyCapRegion r1)) t2).
-Proof. 
- intros.
- unfold tRef. auto.
-Qed.
+ ,  ClosedT t2
+ -> ClosedT (TRef (TCap (TyCapRegion r1)) t2).
+Proof. auto. Qed.
 Hint Resolve closedT_tRef.
 
 
@@ -72,8 +63,8 @@ Hint Resolve closedT_tRef.
 (* Type is well formed under an environment one element larger. *)
 Lemma wfT_succ
  :  forall tn t1
- ,  wfT tn     t1
- -> wfT (S tn) t1.
+ ,  WfT tn     t1
+ -> WfT (S tn) t1.
 Proof.
  intros. gen tn.
  induction t1; intros; inverts H; eauto.
@@ -85,8 +76,8 @@ Hint Resolve wfT_succ.
 Lemma wfT_more
  :  forall tn1 tn2 tt
  ,  tn1 <= tn2
- -> wfT tn1 tt
- -> wfT tn2 tt.
+ -> WfT tn1 tt
+ -> WfT tn2 tt.
 Proof.
  intros. gen tn1 tn2.
  induction tt; intros; inverts H0; eauto.
@@ -105,8 +96,8 @@ Hint Resolve wfT_more.
 (* Type is well formed under a larger environment. *)
 Lemma wfT_max
  :  forall tn1 tn2 tt
- ,  wfT tn1 tt
- -> wfT (max tn1 tn2) tt.
+ ,  WfT tn1 tt
+ -> WfT (max tn1 tn2) tt.
 Proof.
  intros.
  assert (  ((tn1 <  tn2) /\ max tn1 tn2 = tn2) 
@@ -124,7 +115,7 @@ Hint Resolve wfT_max.
 (* For every type, there is an environment that it is well formed under. *)
 Lemma wfT_exists
  :  forall t1
- ,  (exists tn, wfT tn t1).
+ ,  (exists tn, WfT tn t1).
 Proof.
  intros.
  induction t1;
@@ -165,27 +156,4 @@ Proof.
    rewrite Max.max_comm. auto.
 Qed.
 Hint Resolve wfT_exists.
-
-
-(* A type application constructed from well formed components is
-   itself well formed. *)
-Lemma makeTApps_wfT
- :  forall n t1 ts
- ,  wfT n t1 
- -> Forall (wfT n) ts
- -> wfT n (makeTApps t1 ts).
-Proof.
- intros. gen t1.
- induction ts; intros.
-  simpl. auto.
-  simpl.
-  inverts H0.
-  assert (ts = nil \/ (exists t ts', ts = t <: ts')) as HS.
-   apply snocable.
-   inverts HS.
-    simpl. auto. 
-    dest H0. dest H0. subst.
-    eapply IHts. auto.
-     auto.
-Qed.
 
