devel/Iron/SystemF2Effect/Value/Wf.v
@@ -4,91 +4,89 @@ Require Export Iron.SystemF2Effect.Type.
 
 
 (* Well formed expressions are closed under the given environment. *)
-Inductive wfV (kn tn sn: nat) : val -> Prop :=
+Inductive WfV (kn tn sn: nat) : val -> Prop :=
  | WfV_VVar 
    :  forall ti
    ,  ti < tn
-   -> wfV kn tn sn (VVar ti)
+   -> WfV kn tn sn (VVar ti)
  
  | WfV_VLoc
    :  forall li
    ,  li < sn
-   -> wfV kn tn sn (VLoc li) 
+   -> WfV kn tn sn (VLoc li) 
 
  | WfV_VLam
    :  forall t1 x2
-   ,  wfT kn t1 -> wfX kn (S tn) sn x2
-   -> wfV kn tn sn (VLam t1 x2)
+   ,  WfT kn t1 -> WfX kn (S tn) sn x2
+   -> WfV kn tn sn (VLam t1 x2)
 
  | WfV_VLAM
    :  forall k1 x
-   ,  wfX (S kn) tn sn x
-   -> wfV kn tn sn (VLAM k1 x)
+   ,  WfX (S kn) tn sn x
+   -> WfV kn tn sn (VLAM k1 x)
 
  | WfV_VConst
    :  forall c
-   ,  wfV kn tn sn (VConst c)
+   ,  WfV kn tn sn (VConst c)
 
-with   wfX (kn tn sn: nat) : exp -> Prop :=
+with   WfX (kn tn sn: nat) : exp -> Prop :=
 
  | WfX_XVal
    :  forall v
-   ,  wfV kn tn sn v
-   -> wfX kn tn sn (XVal v)
+   ,  WfV kn tn sn v
+   -> WfX kn tn sn (XVal v)
 
  | WfX_XLet 
    :  forall t1 x1 x2
-   ,  wfT kn t1
-   -> wfX kn tn sn x1
-   -> wfX kn (S tn) sn x2
-   -> wfX kn tn sn (XLet t1 x1 x2) 
+   ,  WfT kn t1
+   -> WfX kn tn sn x1
+   -> WfX kn (S tn) sn x2
+   -> WfX kn tn sn (XLet t1 x1 x2) 
 
  | WfX_XApp 
    :  forall v1 v2
-   ,  wfV kn tn sn v1 -> wfV kn tn sn v2
-   -> wfX kn tn sn (XApp v1 v2)
+   ,  WfV kn tn sn v1 -> WfV kn tn sn v2
+   -> WfX kn tn sn (XApp v1 v2)
 
  | WfX_VAPP
    :  forall x1 t2
-   ,  wfV kn tn sn x1 -> wfT kn t2
-   -> wfX kn tn sn (XAPP x1 t2)
+   ,  WfV kn tn sn x1 -> WfT kn t2
+   -> WfX kn tn sn (XAPP x1 t2)
 
  | WfX_XOp1
    :  forall op1 v1
-   ,  wfV kn tn sn v1
-   -> wfX kn tn sn (XOp1 op1 v1)
+   ,  WfV kn tn sn v1
+   -> WfX kn tn sn (XOp1 op1 v1)
 
  | WfX_XNew
    :  forall x
-   ,  wfX (S kn) tn sn x 
-   -> wfX kn     tn sn (XNew x)
+   ,  WfX (S kn) tn sn x 
+   -> WfX kn     tn sn (XNew x)
 
  | WfX_XAlloc
    :  forall tR v1
-   ,  wfT kn tR
-   -> wfV kn tn sn v1
-   -> wfX kn tn sn (XAlloc tR v1)
+   ,  WfT kn tR
+   -> WfV kn tn sn v1
+   -> WfX kn tn sn (XAlloc tR v1)
 
  | WfX_XRead
    :  forall tR v1
-   ,  wfT kn tR
-   -> wfV kn tn sn v1
-   -> wfX kn tn sn (XRead tR v1)
+   ,  WfT kn tR
+   -> WfV kn tn sn v1
+   -> WfX kn tn sn (XRead tR v1)
 
  | WfX_XWrite
    :  forall tR v1 v2
-   ,  wfT kn tR
-   -> wfV kn tn sn v1
-   -> wfV kn tn sn v2
-   -> wfX kn tn sn (XWrite tR v1 v2).
+   ,  WfT kn tR
+   -> WfV kn tn sn v1
+   -> WfV kn tn sn v2
+   -> WfX kn tn sn (XWrite tR v1 v2).
 
-Hint Constructors wfX.
-Hint Constructors wfV.
+Hint Constructors WfX.
+Hint Constructors WfV.
 
 
 (* Closed expressions are well formed under
    empty type and kind environments, but may contain store locations. *)
-Definition closedX (xx: exp) : Prop
- := exists sn, wfX O O sn xx.
-Hint Unfold closedX.
+Notation ClosedX X := (exists sn, WfX O O sn X).
 
